\documentclass[preview]{standalone}
\usepackage[english]{babel}
\usepackage{amsmath}
\usepackage{amssymb}
\begin{document}
\begin{align*}
\begin{align*}
            \int_{-1}^{1} (x^3 - 3x + 2)\, dx
            &= \int_{-1}^{1} x^3 \, dx - 3 \int_{-1}^{1} x \, dx + \int_{-1}^{1} 2 \, dx \\[0.3em]
            &= 0 - 3 \cdot 0 + 2 \cdot \int_{-1}^{1} 1 \, dx \\[0.3em]
            &= 2 \cdot [x]_{-1}^{1} \\[0.3em]
            &= 2 \cdot (1 - (-1)) \\[0.3em]
            &= 2 \cdot 2 = 4
            \end{align*}
\end{align*}
\end{document}